TermTests/CaseOfCaseAndLoopsTest.lean
@@ -37,7 +37,7 @@ local macro:max "run" t:term:max : term => `(Term.run (Sg := sig0) GlobalEnv.nil
 def ifs {Γ : Ctx} {u : Usage Γ} {τ : TyWf} {k : Head} : Term sig0 Γ u τ k → Nat
   | .lam b _ => ifs b
   | .ap f a _ _ => ifs f + ifs a
-  | .letE a b _ _ _ => ifs a + ifs b
+  | .letE a b .. => ifs a + ifs b
   | .bool_casesOn c t e .. => 1 + ifs c + ifs t + ifs e
   | _ => 0
 
@@ -52,7 +52,7 @@ def lamsOfVar {Γ : Ctx} {u : Usage Γ} {τ : TyWf} {k : Head} : Term sig0 Γ u 
 def foldsClosures {Γ : Ctx} {u : Usage Γ} {τ : TyWf} {k : Head} :
     Term sig0 Γ u τ k → Bool
   | .lam b _ => foldsClosures b
-  | .letE a b _ _ _ => foldsClosures a || foldsClosures b
+  | .letE a b .. => foldsClosures a || foldsClosures b
   | .nat_rec _ _ _ (.lam _ _) .. => true
   | .nat_rec _ _ _ b .. => foldsClosures b
   | _ => false
