TermTests/ExternToTermTest.lean
@@ -44,7 +44,7 @@ def externForm? {Γ : Ctx} {u : Usage Γ} {τ : TyWf} {k : Head} :
     Term sig0 Γ u τ k → Option String
   | .lam b _ => externForm? b
   | .ap f a _ _ => externForm? f <|> externForm? a
-  | .letE a b _ _ _ => externForm? a <|> externForm? b
+  | .letE a b .. => externForm? a <|> externForm? b
   | .extern _ _ => some "extern"
   | .externCall _ _ _ _ => some "externCall"
   | .externCallChecked _ _ _ _ _ => some "externCallChecked"
